Finish basic CRC32 spec.

specs/Spec.CRC32.fst
@@ -6,7 +6,7 @@ module U8 = FStar.UInt8
 module UInt = FStar.UInt
 
 open FStar.Seq
-open FStar.Tactics
+open FStar.Mul
 
 val is_rev_refl: (a: U8.t) -> (b: U8.t) -> Lemma
   (ensures is_rev a b <==> is_rev b a)
@@ -27,31 +27,17 @@ let u8_rev v =
 
 let rec seq_append_index_l (#t: Type) (a b: Seq.seq t): Lemma
   (ensures forall i. i < Seq.length a ==> Seq.index a i == Seq.index (a @| b) i)
-  (decreases Seq.length a)
-  [SMTPat (a @| b)] =
+  (decreases Seq.length a) =
   match Seq.length a with
   | 0 -> ()
   | _ -> seq_append_index_l (Seq.tail a) b
 
-// let rec seq_append_index_r (#t: Type) (a b: Seq.seq t): Lemma
-//   (ensures forall i. i < Seq.length b ==> Seq.index (a @| b) (i + Seq.length a) == Seq.index b i)
-//   (decreases Seq.length a)
-//   [SMTPat (a @| b)] =
-//   match Seq.length a with
-//   | 0 -> ()
-//   | _ -> seq_append_index_r (Seq.tail a) b
-
-// #set-options "--z3rlimit 120 --z3seed 1"
-// let logxor_concat (#n: nat{n > 0}) (#m: nat{m > 0}) (a c: BV.bv_t n) (b d: BV.bv_t m):
-//   Lemma (ensures gf2_plus #(n + m) (a @| b) (c @| d) = (a +@ c) @| (b +@ d)) =
-//   let ac = a +@ c in
-//   let bd = b +@ d in
-//   let abcd = gf2_plus #(n + m) (a @| b) (c @| d) in
-//   assert_norm(Seq.length (ac @| bd) == (n + m));
-//   assert_norm(forall (i: nat). i < n ==> Seq.index (ac @| bd) i = Seq.index abcd i);
-//   assert_norm(forall (i: nat). i < m ==> Seq.index (ac @| bd) (n + i) = Seq.index abcd (n + i));
-//   assert_norm(Seq.equal (ac @| bd) abcd)
-// #reset-options
+let rec seq_append_index_r (#t: Type) (a b: Seq.seq t): Lemma
+  (ensures forall i. i < Seq.length b ==> Seq.index (a @| b) (i + Seq.length a) == Seq.index b i)
+  (decreases Seq.length a) =
+  match Seq.length a with
+  | 0 -> ()
+  | _ -> seq_append_index_r (Seq.tail a) b
 
 let logxor_zero_eq (#n: nat{n > 0}) (a: BV.bv_t n): Lemma
   (ensures (BV.logxor_vec a (BV.zero_vec #n)) == a)
@@ -100,7 +86,7 @@ unfold let zero_vec_r (#n: nat{n > 0}) (m: nat) (a: BV.bv_t n): Tot (res: BV.bv_
   | _ -> a @| (BV.zero_vec #m)
 
 unfold let ones_vec_l (#n: nat{n > 0}) (m: nat) (a: BV.bv_t n): Tot (res: BV.bv_t (n + m){
-  forall i. i < m ==> Seq.index res i == true /\
+  forall i. (i < m ==> Seq.index res i == true) /\
     (i >= m /\ i < n + m ==> Seq.index res i == Seq.index a (i - m))
 }) =
   match m with
@@ -134,6 +120,30 @@ unfold let poly_xor (#n: nat{n >= 32}) (a: BV.bv_t n): Tot (res: BV.bv_t n{
   assert(Seq.equal r (Seq.tail r'));
   r
 
+let poly_xor_zero_suffix (#n: nat{n >= 32}) (a: BV.bv_t n) (m: nat) (l: nat): Lemma
+  (ensures forall i. Seq.index (poly_xor (zero_vec_r m a)) i ==
+    Seq.index (poly_xor (zero_vec_r l a)) i) = ()
+
+let rec poly_xor_zero_vec_r (#n: nat{n >= 32}) (a: BV.bv_t n) (m: nat): Lemma
+  (ensures zero_vec_r m (poly_xor a) == poly_xor (zero_vec_r m a)) =
+  match m with
+  | 0 -> ()
+  | _ ->
+    let b = zero_vec_r m (poly_xor a) in
+    let c = poly_xor (zero_vec_r m a) in
+    let b' = zero_vec_r (m - 1) (poly_xor a) in
+    let c' = poly_xor (zero_vec_r (m - 1) a) in
+    poly_xor_zero_suffix a m (m - 1);
+    poly_xor_zero_vec_r a (m - 1);
+    assert(forall i. Seq.index b i == Seq.index b' i);
+    assert(forall i. Seq.index c i == Seq.index c' i);
+    assert(Seq.index b (m + n - 1) == Seq.index c (m + n - 1));
+    assert(Seq.equal b c)
+
+let poly_xor_sub_eq (#n: nat{n > 32}) (a: BV.bv_t n): Lemma
+  (ensures poly_xor #(n - 1) (Seq.tail a) == Seq.tail (a -@ (poly n))) =
+  assert(Seq.equal (poly_xor #(n - 1) (Seq.tail a)) (Seq.tail (a -@ (poly n))))
+
 let poly_xor_aux (#n: nat{n >= 32}) (a b: BV.bv_t n): Lemma
   (ensures (poly_xor a) +@ (poly_xor b) == a +@ b) =
   let p' = Seq.tail (poly (n + 1)) in
@@ -149,18 +159,13 @@ let poly_xor_aux (#n: nat{n >= 32}) (a b: BV.bv_t n): Lemma
     a +@ b;
   }
 
-let rec poly_mod_zero (#n: nat{n > 32}) (a: BV.bv_t n): Lemma
-  (ensures poly_mod #(n + 1) (zero_vec_l 1 a) == poly_mod a) =
-  let a' = zero_vec_l 1 a in
-  assert(Seq.equal (Seq.tail a') a);
+let rec poly_mod_zero (#n: nat{n > 32}) (a: BV.bv_t n {a == BV.zero_vec #n}): Lemma
+  (ensures poly_mod a == BV.zero_vec #32) =
   match n with
-  | 33 -> assert_norm(poly_mod #34 a' == poly_mod #33 (Seq.tail a'))
-  | _ -> poly_mod_zero #(n - 1) (Seq.tail a)
-
-let poly_mod_one (#n: nat{n > 32}) (a: BV.bv_t n): Lemma
-  (ensures poly_mod (ones_vec_l 1 a) == poly_mod (poly_xor a)) =
-  let a' = ones_vec_l 1 a in
-  assert_norm(poly_mod #(n + 1) a' == poly_mod (poly_xor a))
+  | 33 -> assert_norm(Seq.equal (poly_mod a) (BV.zero_vec #32))
+  | _ -> 
+    assert_norm(Seq.equal (Seq.tail a) (BV.zero_vec #(n - 1)));
+    poly_mod_zero #(n - 1) (Seq.tail a)
 
 let rec poly_mod_add (#n: nat{n > 32}) (a b: BV.bv_t n): Lemma
   (ensures (poly_mod a) +@ (poly_mod b) == poly_mod (a +@ b)) =
@@ -238,3 +243,261 @@ let rec poly_mod_add (#n: nat{n > 32}) (a b: BV.bv_t n): Lemma
         poly_mod c;
       }
   end
+
+unfold let magic_matrix_pattern (nzeros: nat{nzeros > 0}) (i: nat{i < 32}):
+  res: BV.bv_t (32 + nzeros){
+    forall j. (j == i ==> Seq.index res j == true) /\ (j <> i ==> Seq.index res j == false)
+  } =
+  let zero_right = BV.zero_vec #(nzeros + 32 - i - 1) in
+  let one = ones_vec_l 1 zero_right in
+  zero_vec_l i one
+
+unfold let is_magic_matrix_elem (nzeros: nat{nzeros > 0}) (i: nat {i < 32}) (v: BV.bv_t 32) =
+  poly_mod (magic_matrix_pattern nzeros i) == v
+
+type matrix_seq = s:Seq.seq (BV.bv_t 32) {length s <= 32}
+
+type sub_matrix_t (nzeros: nat{nzeros > 0}) = m: matrix_seq{
+  forall i. i < Seq.length m ==> is_magic_matrix_elem nzeros i (index m i)
+}
+
+type matrix_t (nzeros: nat{nzeros > 0}) = m: sub_matrix_t nzeros{Seq.length m == 32}
+
+val magic_matrix_init: s: sub_matrix_t 1 -> Tot (matrix_t 1) (decreases 32 - (Seq.length s))
+
+let rec magic_matrix_init s =
+  let l = Seq.length s in
+  if l = 0 then begin
+    let m = ones_vec_l 1 (BV.zero_vec #32) in
+    let n = poly_xor (BV.zero_vec #32) in
+    calc (==) {
+      poly_mod #33 m;
+      =={assert(Seq.head m == true)}
+      Seq.tail (m -@ poly 33);
+      =={}
+      n;
+    };
+    let res = s @| (Seq.create 1 n) in
+    calc (==) {
+      Seq.index res l;
+      =={seq_append_index_r s (Seq.create 1 n)}
+      Seq.index (Seq.create 1 n) 0;
+      =={}
+      n;
+    };
+    magic_matrix_init res
+  end else if l < 32 then begin
+    let n = magic_matrix_pattern 1 l in
+    let res = s @| (Seq.create 1 (poly_mod n)) in
+    calc (==) {
+      Seq.index res l;
+      =={seq_append_index_r s (Seq.create 1 (poly_mod n))}
+      Seq.index (Seq.create 1 (poly_mod n)) 0;
+      =={}
+      poly_mod n;
+    };
+    magic_matrix_init res
+  end else 
+    s
+
+type matrix_dividend (nzeros: nat{nzeros > 0}) = d: BV.bv_t (32 + nzeros) {
+  forall i. i > 31 /\ i < Seq.length d ==> Seq.index d i == false
+}
+
+val bit_extract:
+    #nzeros: nat{nzeros > 0}
+  -> n: matrix_dividend nzeros
+  -> i: nat{i < 32}
+  -> res: BV.bv_t (32 + nzeros) {
+      forall j. (j == i ==> Seq.index res j == Seq.index n j) /\
+        (j <> i ==> Seq.index res j == false)
+    }
+
+let bit_extract #nzeros n i =
+  let zero_right = BV.zero_vec #(nzeros + 32 - i - 1) in
+  let bit = (Seq.create 1 (Seq.index n i)) @| zero_right in
+  zero_vec_l #(nzeros + 32 - i) i bit
+
+val bit_sum:
+    #nzeros: nat{nzeros > 0}
+  -> n: matrix_dividend nzeros
+  -> i: nat{i < 32}
+  -> res: BV.bv_t (32 + nzeros) {
+    forall j. (j <= i ==> Seq.index res j == Seq.index n j) /\ (j > i ==> Seq.index res j == false)
+  }
+
+let rec bit_sum #nzeros n i =
+  match i with
+  | 0 -> bit_extract n i
+  | _ -> (bit_extract n i) +@ (bit_sum n (i - 1))
+
+val do_magic_matrix_times:
+    #nzeros: nat{nzeros > 0}
+  -> m: matrix_t nzeros
+  -> n: BV.bv_t 32
+  -> i: nat{i < 32}
+  -> res: BV.bv_t 32{
+      res == poly_mod (bit_extract (zero_vec_r nzeros n) i)
+    }
+
+let do_magic_matrix_times
+  (#nzeros: nat{nzeros > 0}) (m: matrix_t nzeros) (n: BV.bv_t 32) (i: nat{i < 32}) =
+  if Seq.index n i then begin
+    Seq.index m i
+  end else begin
+    assert(Seq.equal (bit_extract (zero_vec_r nzeros n) i) (BV.zero_vec #(32 + nzeros)));
+    poly_mod_zero (bit_extract (zero_vec_r nzeros n) i);
+    BV.zero_vec #32
+  end
+
+val magic_matrix_times':
+    #nzeros: nat{nzeros > 0}
+  -> m: matrix_t nzeros
+  -> n: BV.bv_t 32
+  -> i: nat{i < 32}
+  -> res: BV.bv_t 32{
+    res == poly_mod (bit_sum (zero_vec_r nzeros n) i)
+  }
+
+let rec magic_matrix_times'
+  (#nzeros: nat{nzeros > 0}) (m: matrix_t nzeros) (n: BV.bv_t 32) (i: nat{i < 32}) =
+  match i with
+  | 0 -> do_magic_matrix_times m n i
+  | _ -> 
+    let n' = do_magic_matrix_times m n i in
+    poly_mod_add (bit_extract (zero_vec_r nzeros n) i) (bit_sum (zero_vec_r nzeros n) (i - 1));
+    n' +@ magic_matrix_times' m n (i - 1)
+
+val magic_matrix_times:
+  #nzeros: nat {nzeros > 0} ->
+  matrix_t nzeros ->
+  n: BV.bv_t 32 ->
+  res: BV.bv_t 32 {res == poly_mod (zero_vec_r nzeros n)}
+
+let magic_matrix_times #nzeros m n =
+  assert_norm(Seq.equal (bit_sum (zero_vec_r nzeros n) 31) (zero_vec_r nzeros n));
+  magic_matrix_times' m n 31
+
+#set-options "--z3rlimit 200"
+let rec poly_mod_zero_suffix (#n: nat{n > 32}) (a: BV.bv_t n) (m: nat{m > 0}): Lemma
+  (ensures poly_mod (zero_vec_r m (poly_mod a)) == poly_mod (zero_vec_r m a)) =
+  assert(Seq.equal (zero_vec_r #(n - 1) m (Seq.tail a)) (Seq.tail (zero_vec_r m a)));
+  if n = 33 then
+    if Seq.index a 0 then
+      calc (==) {
+        poly_mod (zero_vec_r m (poly_mod a));
+        =={assert(Seq.equal (poly_mod a) (poly_xor #(n - 1) (Seq.tail a)))}
+        poly_mod (zero_vec_r m (poly_xor #(n - 1) (Seq.tail a)));
+        =={
+          let left = (zero_vec_r m (poly_xor #(n - 1) (Seq.tail a))) in
+          let right = (poly_xor #(n + m - 1) (Seq.tail (zero_vec_r m a))) in
+          assert(Seq.equal left right)
+        }
+        poly_mod (poly_xor #(n + m - 1) (Seq.tail (zero_vec_r m a)));
+        =={poly_xor_sub_eq (zero_vec_r m a)}
+        poly_mod (zero_vec_r m a);
+      }
+    else
+      calc (==) {
+        poly_mod (zero_vec_r m (poly_mod a));
+        =={}
+        poly_mod (zero_vec_r #(n - 1) m (Seq.tail a));
+        =={}
+        poly_mod #(n + m - 1) (Seq.tail (zero_vec_r m a));
+        =={}
+        poly_mod (zero_vec_r m a);
+      }
+  else
+    if Seq.index a 0 then
+      calc (==) {
+        poly_mod (zero_vec_r m (poly_mod a));
+        =={}
+        poly_mod (zero_vec_r m (poly_mod #(n - 1) (Seq.tail (a -@ (poly n)))));
+        =={poly_xor_sub_eq a}
+        poly_mod (zero_vec_r m (poly_mod (poly_xor #(n - 1) (Seq.tail a))));
+        =={poly_mod_zero_suffix (poly_xor #(n - 1) (Seq.tail a)) m}
+        poly_mod (zero_vec_r m (poly_xor #(n - 1) (Seq.tail a)));
+        =={poly_xor_zero_vec_r #(n - 1) (Seq.tail a) m}
+        poly_mod (poly_xor (zero_vec_r #(n - 1) m (Seq.tail a)));
+        =={}
+        poly_mod (poly_xor #(n + m - 1) (Seq.tail (zero_vec_r m a)));
+        =={poly_xor_sub_eq (zero_vec_r m a)}
+        poly_mod (zero_vec_r m a);
+      }
+    else
+      calc (==) {
+        poly_mod (zero_vec_r m (poly_mod a));
+        =={}
+        poly_mod (zero_vec_r m (poly_mod #(n - 1) (Seq.tail a)));
+        =={poly_mod_zero_suffix #(n - 1) (Seq.tail a) m}
+        poly_mod (zero_vec_r #(n - 1) m (Seq.tail a));
+        =={}
+        poly_mod #(n + m - 1) (Seq.tail (zero_vec_r m a));
+        =={}
+        poly_mod (zero_vec_r m a);
+      }
+
+let magic_matrix_times_double
+  (#nzeros: nat{nzeros > 0}) (m: matrix_t nzeros) (i: nat{i < 32}): Lemma
+  (ensures is_magic_matrix_elem (nzeros * 2) i (magic_matrix_times m (Seq.index m i))) =
+  let p = magic_matrix_pattern nzeros i in
+  let p' = magic_matrix_pattern (nzeros * 2) i in
+  let p'' = zero_vec_r nzeros p in
+  let n = magic_matrix_times m (Seq.index m i) in
+  poly_mod_zero_suffix p nzeros;
+  assert(forall j.{:pattern Seq.index p' j} j < 32 + nzeros ==> Seq.index p j == Seq.index p' j);
+  assert(forall j.{:pattern Seq.index p'' j} j < 32 + nzeros ==> Seq.index p j == Seq.index p'' j);
+  assert(forall j.{:pattern Seq.index p' j} j >= 32 + nzeros ==> Seq.index p' j == false);
+  assert(forall j.{:pattern Seq.index p'' j} j >= 32 + nzeros ==> Seq.index p'' j == false);
+  assert(Seq.equal p'' p');
+  calc (==) {
+    n;
+    =={}
+    poly_mod (zero_vec_r nzeros (Seq.index m i));
+    =={}
+    poly_mod (zero_vec_r nzeros (poly_mod p));
+    =={}
+    poly_mod (zero_vec_r nzeros p);
+    =={}
+    poly_mod p';
+    =={}
+    poly_mod (magic_matrix_pattern (nzeros * 2) i);
+  }
+
+val magic_matrix_square':
+    #nzeros: nat{nzeros > 0}
+  -> m: matrix_t nzeros
+  -> s: sub_matrix_t (nzeros * 2)
+  -> Tot (matrix_t (nzeros * 2))
+    (decreases 32 - (Seq.length s))
+
+let rec magic_matrix_square' #nzeros m s =
+  if Seq.length s < 32 then begin
+    magic_matrix_times_double m (Seq.length s);
+    let n: BV.bv_t 32 = magic_matrix_times m (Seq.index m (Seq.length s)) in
+    let res = s @| (Seq.create 1 n) in
+    seq_append_index_r s (Seq.create 1 n);
+    calc (==) {
+      poly_mod (magic_matrix_pattern (nzeros * 2) (Seq.length s));
+      =={}
+      n;
+      =={}
+      Seq.index (Seq.create 1 n) 0;
+      =={}
+      Seq.index res (Seq.length s);
+    };
+    assert(forall i.{:pattern Seq.index res i}
+      i < Seq.length s ==> Seq.index res i == Seq.index s i);
+    assert(forall i. i < Seq.length res ==> is_magic_matrix_elem (nzeros * 2) i (Seq.index res i));
+    magic_matrix_square' #nzeros m res
+  end
+  else
+    s
+
+val magic_matrix_square:
+    #nzeros: nat {nzeros > 0}
+  -> matrix_t nzeros
+  -> Tot (matrix_t (nzeros * 2))
+
+let magic_matrix_square #_ m =
+  magic_matrix_square' m (Seq.empty #(BV.bv_t 32))
